src/Pipit.System.Exp.Properties.fst
@@ -1,54 +1,323 @@
 (* Shelved - translation to transition system proof *)
 module Pipit.System.Exp.Properties
 
+module C = Pipit.Context
 
 open Pipit.System.Base
 open Pipit.System.Exp
+open Pipit.System.Det
 
+open Pipit.Exp
+
+#push-options "--split_queries always"
+#push-options "--fuel 1 --ifuel 1"
+
+(*
+   The invariant describes the transition system's state after it has been fed with all of `rows` as inputs.
+   It probably doesn't need to take the bigstep relation as input, as we could just
+   synthesise it with lemma_bigstep_total as required. In fact, we need to
+   synthesise it anyway in some cases.
+*)
 // let rec system_of_exp_invariant
-//   (#outer #vars: nat)
-//   (e: exp { wf e vars /\ causal e })
-//   (streams: C.table outer vars)
-//   (vs: C.vector value outer)
-//   (hBS: bigstep streams e vs)
+//   (rows: list (C.row 'c) { Cons? rows })
+//   (e: exp 'c 'a { causal e })
+//   (v: 'a)
+//   (hBS: bigstep rows e v)
 //   (s: state_of_exp e):
 //     Tot prop (decreases e) =
 //   match e with
-//   | XVar _ -> unit
 //   | XVal _ -> unit
-//   | XPrim2 _ e1 e2 ->
-//     let (s1, s2) = s <: (state_of_exp e1 * state_of_exp e2) in
-//     let BSPrim2 _ _ _ _ vs1 vs2 hBS1 hBS2 = hBS in
-//     system_of_exp_invariant e1 streams vs1 hBS1 s1 /\
-//     system_of_exp_invariant e2 streams vs2 hBS2 s2
-//   | XPre e1 ->
-//     begin
-//     match hBS with
-//       | BSPre0 e -> True
-//       | BSPre _ _ _ vs1 hBS1 ->
-//     let v1'   = bigstep_monotone_inv_next #(outer - 1) #vars #streams hBS1 in
-//     let hBS1' = bigstep_monotone_inv #(outer - 1) #vars #streams hBS1 in
-//     let (s1, v1) = s <: (state_of_exp e1 * value) in
-//     (system_of_exp_invariant #outer #vars e1 streams (v1' :: vs1) hBS1' s1 /\ v1 == v1')
-//   end
+//   | XVar _ -> false_elim ()
+//   | XBVar _ -> unit
+//   | XApp e1 e2 ->
+//     assert_norm (causal (XApp e1 e2) == (causal e1 && causal e2));
+//     assert_norm (state_of_exp (XApp e1 e2) == (state_of_exp e1 & state_of_exp e2));
+//     let s: state_of_exp e1 & state_of_exp e2 = s in
+//     let (s1, s2) = s in
+//     let BSApp _ _ _ v1 v2 hBS1 hBS2 = hBS in
+//     system_of_exp_invariant rows e1 v1 hBS1 s1 /\
+//     system_of_exp_invariant rows e2 v2 hBS2 s2
+
+//   | XFby v1 e2 ->
+//     let s: state_of_exp e2 & 'a = s in
+//     let (s1, v_buf) = s in
+//     let (| v', hBS1' |) = lemma_bigstep_total rows e2 in
+//     v_buf == v' /\ system_of_exp_invariant rows e2 v' hBS1' s1
 
 //   | XThen e1 e2 ->
-//     let (init, s2) = coerce_eq #_ #(bool * state_of_exp e2) () s in
-//     let BSThen _ _ _ vs1 vs2 hBS1 hBS2 = hBS in
-//     (init = (outer > 0)) /\ system_of_exp_invariant e2 streams vs2 hBS2 s2
-//   | XMu e1 ->
-//     let s1 = coerce_eq #_ #(state_of_exp e1) () s in
-//     let BSMu _ _ vs1 hBS1 = hBS in
-//     let hBS' = bigstep_substitute_XMu e1 streams vs hBS in
-//     system_of_exp_invariant #outer #(vars + 1) e1 (C.table_map_append (C.table_of_values vs1) streams) vs1 hBS' s1
+//     let s: system_then_state (state_of_exp e1) (state_of_exp e2) = s in
+//     let (| v1, hBS1' |) = lemma_bigstep_total rows e1 in
+//     let (| v2, hBS2' |) = lemma_bigstep_total rows e2 in
 
-// TODO temp disable proof while simplifying transform
-// let rec step0_ok
-//   (#vars: nat)
-//   (e: exp { causal e /\ wf e vars })
-//   (row: C.row vars)
-//   (v: value)
-//   (hBS: bigstep (C.Table [row]) e [v]):
+//     (s.init == false /\ // (List.Tot.length rows = 0) /\
+//         system_of_exp_invariant rows e1 v1 hBS1' s.s1 /\
+//         system_of_exp_invariant rows e2 v2 hBS2' s.s2)
+
+//   | XMu _ e1 ->
+//     let s: state_of_exp e1 = coerce_eq () s in
+//     let (| vs, hBSmus |) = lemma_bigsteps_total rows e in
+//     let BSsS _ _ _ _ _ _ hBSmu = hBSmus in
+//     bigstep_deterministic hBS hBSmu;
+//     assert (v == List.Tot.hd vs);
+
+//     let rows' = C.row_zip2_cons vs rows in
+//     let hBS' = lemma_bigstep_substitute_elim_XMu rows e1 vs hBSmus in
+//     system_of_exp_invariant rows' e1 v hBS' s
+
+//   | XLet b e1 e2 ->
+//     let s: state_of_exp e1 & state_of_exp e2 = s in
+//     let (s1, s2) = s in
+//     let (| vlefts, hBSlefts |) = lemma_bigsteps_total rows e1 in
+//     let BSsS _ _ _ _ _ _ hBSleft = hBSlefts in
+//     let rows' = C.row_zip2_cons vlefts rows in
+//     let hBS': bigstep rows' e2 v = lemma_bigstep_substitute_elim_XLet rows e1 vlefts hBSlefts e2 v hBS in
+//     system_of_exp_invariant rows e1 (List.Tot.hd vlefts) hBSleft s1 /\
+//       system_of_exp_invariant rows' e2 v hBS' s2
+
+//   | XCheck _ e1 e2 ->
+//     let s: (xprop & state_of_exp e1) & state_of_exp e2 = s in
+//     let ((xp, s1), s2) = s in
+//     let (| v1, hBS1 |) = lemma_bigstep_total rows e1 in
+//     let BSCheck _ _ _ _ _ hBS2 = hBS in
+//     system_of_exp_invariant rows e1 v1 hBS1 s1 /\
+//       system_of_exp_invariant rows e2 v hBS2 s2
+
+let rec system_of_exp_invariant
+  (rows: list (C.row 'c) { Cons? rows })
+  (e: exp 'c 'a { causal e })
+  (s: state_of_exp e):
+    Tot prop (decreases e) =
+  match e with
+  | XVal _ -> True
+  | XVar _ -> false_elim ()
+  | XBVar _ -> True
+  | XApp e1 e2 ->
+    assert_norm (causal (XApp e1 e2) == (causal e1 && causal e2));
+    assert_norm (state_of_exp (XApp e1 e2) == (state_of_exp e1 & state_of_exp e2));
+    let s: state_of_exp e1 & state_of_exp e2 = s in
+    let (s1, s2) = s in
+    system_of_exp_invariant rows e1 s1 /\
+    system_of_exp_invariant rows e2 s2
+
+  | XFby v1 e2 ->
+    let s: state_of_exp e2 & 'a = s in
+    let (s1, v_buf) = s in
+    let v = lemma_bigstep_total_v rows e2 in
+    v_buf == v /\ system_of_exp_invariant rows e2 s1
+
+  | XThen e1 e2 ->
+    let s: system_then_state (state_of_exp e1) (state_of_exp e2) = s in
+    (s.init == false /\
+        system_of_exp_invariant rows e1 s.s1 /\
+        system_of_exp_invariant rows e2 s.s2)
+
+  | XMu _ e1 ->
+    let s: state_of_exp e1 = coerce_eq () s in
+    let (| vs, hBSmus |) = lemma_bigsteps_total rows e in
+    let rows' = C.row_zip2_cons vs rows in
+    system_of_exp_invariant rows' e1 s
+
+  | XLet b e1 e2 ->
+    let s: state_of_exp e1 & state_of_exp e2 = s in
+    let (s1, s2) = s in
+    let (| vlefts, hBSlefts |) = lemma_bigsteps_total rows e1 in
+    let rows' = C.row_zip2_cons vlefts rows in
+    system_of_exp_invariant rows e1 s1 /\
+      system_of_exp_invariant rows' e2 s2
+
+  | XCheck _ e1 e2 ->
+    let s: (xprop & state_of_exp e1) & state_of_exp e2 = s in
+    let ((xp, s1), s2) = s in
+    system_of_exp_invariant rows e1 s1 /\
+      system_of_exp_invariant rows e2 s2
+
+// let dsystem_of_exp_invariant'
+//   (rows: list (C.row 'c))
+//   (e: exp 'c 'a { causal e })
+//   (s: state_of_exp e):
+//     prop =
+//   match rows with
+//   | [] -> s == (dsystem_of_exp e).init
+//   | _ :: _ ->
+//     let (| v, hBS |) = lemma_bigstep_total rows e in
+//     system_of_exp_invariant rows e v hBS s
+
+// let dsystem_of_exp_agrees
+//   (rows: list (C.row 'c))
+//   (e: exp 'c 'a { causal e })
+//   (s0: option (state_of_exp e))
+//   (row: C.row 'c)
+//   (v: 'a) =
+//  let t = dsystem_of_exp e in
+//  let s0' =
+//     match s0 with
+//     | None -> t.init
+//     | Some s0' -> s0'
+//  in
+//  let pre =
+//    match s0 with
+//    | None -> state_of_exp_invariant rows e v s0'
+
+
+// let rec dstep0_ok
+//   (row: C.row 'c)
+//   (e: exp 'c 'a { causal e }):
+//     Lemma (ensures (
+//       let t = dsystem_of_exp e in
+//       let (s', v') = t.step row t.init in
+//       v' == (lemma_bigstep_total_v [row] e) /\ system_of_exp_invariant [row] e s'))
+//         (decreases e) =
+//   match e with
+//   | XVal _ -> ()
+//   | XBVar _ -> ()
+//   | XVar _ -> false_elim ()
+//   | XApp e1 e2 ->
+//     assert_norm (causal (XApp e1 e2) == (causal e1 && causal e2));
+//     assert_norm (state_of_exp (XApp e1 e2) == (state_of_exp e1 & state_of_exp e2));
+//     let t1 = dsystem_of_exp e1 in
+//     let t2 = dsystem_of_exp e2 in
+//     let t  = dsystem_ap2 t1 t2 in
+//     assert_norm (dsystem_of_exp (XApp e1 e2) == t);
+//     dstep0_ok row e1;
+//     dstep0_ok row e2;
+//     let (s', v') = t.step row t.init in
+//     assert (system_of_exp_invariant [row] e1 (fst s'));
+//     assert (system_of_exp_invariant [row] e2 (snd s'));
+//     assert_norm (system_of_exp_invariant [row] (XApp e1 e2) s');
+//     let (|v, hBS |) = lemma_bigstep_total [row] e in
+//     (match hBS with
+//     | BSApp _ _ _ _ _ _ _ -> ());
+//     assert (v' == v);
+//     admit ()
+//   | XFby v1 e2 ->
+//     let (| v2, hBS2 |) = lemma_bigstep_total [row] e2 in
+//     dstep0_ok row e2
+//   | XThen e1 e2 ->
+//     assert_norm (List.Tot.length [row] == 1);
+//     let t1 = dsystem_of_exp e1 in
+//     let t2 = dsystem_of_exp e2 in
+//     let t = dsystem_then t1 t2 in
+//     assert_norm (dsystem_of_exp (XThen e1 e2) == t);
+//     // dstep0_ok row e1;
+//     // dstep0_ok row e2;
+//     // let (s', v') = t.step row t.init in
+//     // assert (system_of_exp_invariant [row] e1 s'.s1);
+//     // assert (system_of_exp_invariant [row] e2 s'.s2);
+//     // assert_norm (system_of_exp_invariant [row] (XThen e1 e2) s');
+//     admit ()
+
+//   | _ -> admit ()
+
+
+
+let rec dstep0_ok
+    (row: C.row 'c)
+    (e: exp 'c 'a { causal e })
+    (v: 'a)
+    (hBS: bigstep [row] e v):
+      Lemma (ensures (
+        let t = dsystem_of_exp e in
+        let (s', v') = t.step row t.init in
+        v == v' /\ system_of_exp_invariant [row] e s'))
+          (decreases e) =
+    match e with
+    | XVal _ -> ()
+    | XBVar _ -> ()
+    | XVar _ -> false_elim ()
+    | XApp e1 e2 ->
+      assert_norm (causal (XApp e1 e2) == (causal e1 && causal e2));
+      assert_norm (state_of_exp (XApp e1 e2) == (state_of_exp e1 & state_of_exp e2));
+      let t1 = dsystem_of_exp e1 in
+      let t2 = dsystem_of_exp e2 in
+      let t  = dsystem_ap2 t1 t2 in
+      assert_norm (dsystem_of_exp (XApp e1 e2) == t);
+      let BSApp _ _ _ v1 v2 hBS1 hBS2 = hBS in
+      dstep0_ok row e1 v1 hBS1;
+      dstep0_ok row e2 v2 hBS2;
+      let (s', v') = t.step row t.init in
+      assert_norm (system_of_exp_invariant [row] (XApp e1 e2) s')
+    | XFby v1 e2 ->
+      let (| v2, hBS2 |) = lemma_bigstep_total [row] e2 in
+      dstep0_ok row e2 v2 hBS2
+    | XThen e1 e2 ->
+      assert_norm (List.Tot.length [row] == 1);
+      let BSThen1 _ _ _ _ hBS1 = hBS in
+      let (| v2, hBS2 |) = lemma_bigstep_total [row] e2 in
+      let t1 = dsystem_of_exp e1 in
+      let t2 = dsystem_of_exp e2 in
+      let t = dsystem_then t1 t2 in
+      assert_norm (dsystem_of_exp (XThen e1 e2) == t);
+      dstep0_ok row e1 v hBS1;
+      dstep0_ok row e2 v2 hBS2;
+      let (s', v') = t.step row t.init in
+      assert (system_of_exp_invariant [row] e1 s'.s1);
+      assert (system_of_exp_invariant [row] e2 s'.s2);
+      assert (s'.init == false);
+      // assert (system_of_exp_invariant [row] (XThen e1 e2) s');
+      ()
+
+    | XMu _ e1 ->
+      let t1 = dsystem_of_exp e1 in
+      let t = dsystem_mu_causal #(C.row 'c) #('a & C.row 'c) (fun i v -> (v, i)) t1 in
+
+      let bottom = Pipit.Inhabited.get_inhabited <: 'a in
+      let (s_scrap, v0) = t1.step (bottom, row) t1.init in
+      let (s1', v') = t1.step (v0, row) t1.init in
+
+      let hBSs0: bigsteps [] (XMu e1) [] = BSs0 (XMu e1) in
+      let (|v0x, hBSX |) = lemma_bigstep_total [C.row_cons bottom row] e1 in
+      let hBSMu: bigstep [row] (XMu e1) v0x = lemma_bigstep_substitute_intros_XMu [] e1 [] row v0x bottom hBSs0 hBSX in
+      let hBSMus: bigsteps [row] (XMu e1) [v0x] = BSsS _ _ _ _ _ hBSs0 hBSMu in
+
+      dstep0_ok (C.row_cons bottom row) e1 v0x hBSX;
+      assert (v0 == v0x);
+      let hBSX': bigstep [C.row_cons v0x row] e1 v0x = lemma_bigstep_substitute_elim_XMu [row] e1 [v0x] hBSMus
+        in
+
+      dstep0_ok (C.row_cons v0x row) e1 v0x hBSX';
+      assert (v' == v0x);
+      bigstep_deterministic hBSMu hBS;
+      assert (v == v0x);
+
+      assert (t.step row t.init == (s1', v'));
+
+      assert (system_of_exp_invariant [C.row_cons v0x row] e1 s1');
+      let s1'': state_of_exp (XMu e1) = coerce_eq () s1' in
+      let (| vs''', hBSmus''' |) = lemma_bigsteps_total [row] e in
+      (match hBSmus''' with | BSsS _ _ _ _ _ (BSs0 _) hBSMu''' ->
+        bigstep_deterministic hBSMu''' hBSMu);
+      assume ([C.row_cons v0x row] == C.row_zip2_cons vs''' [row]);
+      assert (system_of_exp_invariant [row] (XMu e1) s1'');
+      ()
+
+
+//   | XMu _ e1 ->
+//     let s: state_of_exp e1 = coerce_eq () s in
+//     let (| vs, hBSmus |) = lemma_bigsteps_total rows e in
+//     let BSsS _ _ _ _ _ _ hBSmu = hBSmus in
+//     bigstep_deterministic hBS hBSmu;
+//     assert (v == List.Tot.hd vs);
+
+//     let rows' = C.row_zip2_cons vs rows in
+//     let hBS' = lemma_bigstep_substitute_elim_XMu rows e1 vs hBSmus in
+//     system_of_exp_invariant rows' e1 v hBS' s
+
+//   | XLet b e1 e2 ->
+//     let s: state_of_exp e1 & state_of_exp e2 = s in
+//     let (s1, s2) = s in
+//     let (| vlefts, hBSlefts |) = lemma_bigsteps_total rows e1 in
+//     let BSsS _ _ _ _ _ _ hBSleft = hBSlefts in
+//     let rows' = C.row_zip2_cons vlefts rows in
+//     let hBS': bigstep rows' e2 v = lemma_bigstep_substitute_elim_XLet rows e1 vlefts hBSlefts e2 v hBS in
+//     system_of_exp_invariant rows e1 (List.Tot.hd vlefts) hBSleft s1 /\
+//       system_of_exp_invariant rows' e2 v hBS' s2
+
+
+    | _ -> admit ()
+
+
+
+
 //     Tot (s': state_of_exp e & u: unit { system_of_exp e vars row None s' v /\ system_of_exp_invariant #0 e (C.Table [row]) [v] hBS s' }) (decreases e) =
 //   let streams = (C.Table #1 #vars [row]) in
 //   match e with
