src/Pipit.Exp.fst
@@ -1,6 +1,6 @@
 module Pipit.Exp
 
 include Pipit.Exp.Base
-include Pipit.Exp.Subst
+include Pipit.Exp.Binding
 include Pipit.Exp.Bigstep
 include Pipit.Exp.Causality
